proof/crefine/SR_lemmas_C.thy
@@ -1120,7 +1120,7 @@ lemma rf_sr_upd:
   unfolding rf_sr_def using assms
   by simp (rule cstate_relation_only_t_hrs, auto)
 
-lemma rf_sr_upd_safe [simp]:
+lemma rf_sr_upd_safe[simp]:
   assumes rl: "(t_hrs_' (globals (g y))) = (t_hrs_' (globals y))"
   and     rq: "(ksReadyQueues_' (globals (g y))) = (ksReadyQueues_' (globals y))"  
   and     sa: "(ksSchedulerAction_' (globals (g y))) = (ksSchedulerAction_' (globals y))"
@@ -1977,6 +1977,16 @@ lemma ghost_assertion_size_logic:
     \<Longrightarrow> gs_get_assn cap_get_capSizeBits_'proc (ghost'state_' (globals \<sigma>)) = 0 \<or>
             sz \<le> gs_get_assn cap_get_capSizeBits_'proc (ghost'state_' (globals \<sigma>))"
   by (clarsimp simp: rf_sr_def ghost_assertion_size_logic')
+
+lemma gs_set_assn_Delete_cstate_relation:
+  "cstate_relation s (ghost'state_'_update (gs_set_assn cteDeleteOne_'proc v) gs)
+    = cstate_relation s gs"
+  apply (cases "ghost'state_' gs")
+  apply (auto simp: rf_sr_def cstate_relation_def Let_def carch_state_relation_def
+                    cmachine_state_relation_def ghost_assertion_data_set_def
+                    ghost_size_rel_def ghost_assertion_data_get_def
+                    cteDeleteOne_'proc_def cap_get_capSizeBits_'proc_def)
+  done
 
 end
 end
